Prefix(:=<http://emmc.info/emmo-granularity#>)
Prefix(owl:=<http://www.w3.org/2002/07/owl#>)
Prefix(rdf:=<http://www.w3.org/1999/02/22-rdf-syntax-ns#>)
Prefix(xml:=<http://www.w3.org/XML/1998/namespace>)
Prefix(xsd:=<http://www.w3.org/2001/XMLSchema#>)
Prefix(rdfs:=<http://www.w3.org/2000/01/rdf-schema#>)


Ontology(<http://emmc.info/emmo-granularity>
Import(<http://emmc.info/emmo-physical>)
Annotation(<http://emmc.info/emmo-core#EMMO_5525a055_dda5_4556_8b91_f0d22fa676cc> "EMMO is released under a Creative Commons license Attribution 4.0 International (CC BY 4.0)

https://creativecommons.org/licenses/by/4.0/legalcode")
Annotation(<http://emmc.info/emmo-core#EMMO_cd5fb112_7ee7_4120_a35d_3ca3e6c3f4ab> "Emanuele Ghedini (University of Bologna, IT)
Gerhard Goldbeck (GCL Ltd, UK)
Adham Hashibon (Fraunhofer IWM, DE)
Georg Schmitz (Access, DE)
Jesper Friis (SINTEF, NO)")
Annotation(rdfs:comment "Contacts:
Gerhard Goldbeck
Goldbeck Consulting Ltd (UK)
email: gerhard@goldbeck-consulting.com

Emanuele Ghedini
University of Bologna (IT)
email: emanuele.ghedini@unibo.it")
Annotation(rdfs:comment "European Materials and Modelling Ontology (EMMO)

EMMO is a multidisciplinary effort to develop a standard representational framework (the ontology) based on current materials modelling knowledge, including physical sciences, analytical philosophy and information and communication technologies. 

It provides the connection between the physical world, materials characterisation world and materials modelling world.")
Annotation(rdfs:comment "The EMMO requires FaCT++ reasoner plugin in order to visualize all inferences and class hierarchy (ctrl+R hotkey in Protege).")
Annotation(owl:versionInfo "The European Materials Modelling Ontology

Version 0.9.10")

Declaration(Class(<http://emmc.info/emmo-core#EMMO_0f795e3e_c602_4577_9a43_d5a231aa1360>))
Declaration(Class(<http://emmc.info/emmo-core#EMMO_c5ddfdba_c074_4aa4_ad6b_1ac4942d300d>))
Declaration(Class(<http://emmc.info/emmo-direct#EMMO_36c79456_e29c_400d_8bd3_0eedddb82652>))
Declaration(Class(<http://emmc.info/emmo-direct#EMMO_52211e5e_d767_4812_845e_eb6b402c476a>))
Declaration(ObjectProperty(<http://emmc.info/emmo-direct#EMMO_65a2c5b8_e4d8_4a51_b2f8_e55effc0547d>))
Declaration(ObjectProperty(<http://emmc.info/emmo-direct#EMMO_a50d920d_1ee3_4668_9a73_5d80a1c6fe15>))
Declaration(ObjectProperty(<http://emmc.info/emmo-direct#EMMO_b2282816_b7a3_44c6_b2cb_3feff1ceb7fe>))

############################
#   Object Properties
############################

# Object Property: <http://emmc.info/emmo-direct#EMMO_65a2c5b8_e4d8_4a51_b2f8_e55effc0547d> (has_temporal_direct_part)

AnnotationAssertion(rdfs:label <http://emmc.info/emmo-direct#EMMO_65a2c5b8_e4d8_4a51_b2f8_e55effc0547d> "has_temporal_direct_part"@en)
SubObjectPropertyOf(<http://emmc.info/emmo-direct#EMMO_65a2c5b8_e4d8_4a51_b2f8_e55effc0547d> <http://emmc.info/emmo-core#EMMO_7afbed84_7593_4a23_bd88_9d9c6b04e8f6>)
InverseFunctionalObjectProperty(<http://emmc.info/emmo-direct#EMMO_65a2c5b8_e4d8_4a51_b2f8_e55effc0547d>)
AsymmetricObjectProperty(<http://emmc.info/emmo-direct#EMMO_65a2c5b8_e4d8_4a51_b2f8_e55effc0547d>)
IrreflexiveObjectProperty(<http://emmc.info/emmo-direct#EMMO_65a2c5b8_e4d8_4a51_b2f8_e55effc0547d>)

# Object Property: <http://emmc.info/emmo-direct#EMMO_a50d920d_1ee3_4668_9a73_5d80a1c6fe15> (has_direct_part)

AnnotationAssertion(rdfs:label <http://emmc.info/emmo-direct#EMMO_a50d920d_1ee3_4668_9a73_5d80a1c6fe15> "has_direct_part"@en)
SubObjectPropertyOf(<http://emmc.info/emmo-direct#EMMO_a50d920d_1ee3_4668_9a73_5d80a1c6fe15> <http://emmc.info/emmo-core#EMMO_9380ab64_0363_4804_b13f_3a8a94119a76>)
InverseFunctionalObjectProperty(<http://emmc.info/emmo-direct#EMMO_a50d920d_1ee3_4668_9a73_5d80a1c6fe15>)
AsymmetricObjectProperty(<http://emmc.info/emmo-direct#EMMO_a50d920d_1ee3_4668_9a73_5d80a1c6fe15>)
IrreflexiveObjectProperty(<http://emmc.info/emmo-direct#EMMO_a50d920d_1ee3_4668_9a73_5d80a1c6fe15>)

# Object Property: <http://emmc.info/emmo-direct#EMMO_b2282816_b7a3_44c6_b2cb_3feff1ceb7fe> (has_spatial_direct_part)

AnnotationAssertion(rdfs:label <http://emmc.info/emmo-direct#EMMO_b2282816_b7a3_44c6_b2cb_3feff1ceb7fe> "has_spatial_direct_part"@en)
SubObjectPropertyOf(<http://emmc.info/emmo-direct#EMMO_b2282816_b7a3_44c6_b2cb_3feff1ceb7fe> <http://emmc.info/emmo-4d#EMMO_f68030be_94b8_4c61_a161_886468558054>)
InverseFunctionalObjectProperty(<http://emmc.info/emmo-direct#EMMO_b2282816_b7a3_44c6_b2cb_3feff1ceb7fe>)
AsymmetricObjectProperty(<http://emmc.info/emmo-direct#EMMO_b2282816_b7a3_44c6_b2cb_3feff1ceb7fe>)
IrreflexiveObjectProperty(<http://emmc.info/emmo-direct#EMMO_b2282816_b7a3_44c6_b2cb_3feff1ceb7fe>)



############################
#   Classes
############################

# Class: <http://emmc.info/emmo-core#EMMO_0f795e3e_c602_4577_9a43_d5a231aa1360> (elementary)

SubClassOf(<http://emmc.info/emmo-core#EMMO_0f795e3e_c602_4577_9a43_d5a231aa1360> <http://emmc.info/emmo-direct#EMMO_36c79456_e29c_400d_8bd3_0eedddb82652>)

# Class: <http://emmc.info/emmo-direct#EMMO_36c79456_e29c_400d_8bd3_0eedddb82652> (state)

AnnotationAssertion(<http://emmc.info/emmo-core#EMMO_967080e5_2f42_4eb2_a3a9_c58143e835f9> <http://emmc.info/emmo-direct#EMMO_36c79456_e29c_400d_8bd3_0eedddb82652> "A 'physical' whose spatial direct parts extends from one change in spatial direct part cardinality (i.e. the number of spatial direct parts) to the immidiate next change.")
AnnotationAssertion(<http://emmc.info/emmo-core#EMMO_b432d2d5_25f4_4165_99c5_5935a7763c1a> <http://emmc.info/emmo-direct#EMMO_36c79456_e29c_400d_8bd3_0eedddb82652> "e.g. the existent in my glass is declared at t = t_start as made of two direct parts: the ice and the water. It will continue to exists as state as long as the ice is completely melt at t = t_end. The new state will be completely made of water. Between t_start and t_end there is an exchange of molecules between the ice and the water, but this does not affect the existence of the two states.

If we partition the existent in my glass as ice surrounded by several molecules (we do not use the object water as direct part) then the appearance of a molecule coming from the ice will cause a state to end and another state to begin.")
AnnotationAssertion(rdfs:comment <http://emmc.info/emmo-direct#EMMO_36c79456_e29c_400d_8bd3_0eedddb82652> "Direct partitions declaration is a choice of the ontology developer that choses the classes to be used as direct parts, according to its own world view.

A 'state' can always be direct partitioned in 'elementary'-s and 'void' or 'physical'.

e.g. the water in my glass can be seen as a single object without declaring direct parts, or as made of H2O molecules direct parts.")
AnnotationAssertion(rdfs:comment <http://emmc.info/emmo-direct#EMMO_36c79456_e29c_400d_8bd3_0eedddb82652> "The definition of 'state' implies that its direct parts (i.e. 'physicals') are not gained or lost during its temporal extension (they exist from the left to the right side of the time interval), so that the granularity of a 'state' is constant.

This does not mean that there cannot be a change in the internal structure of the 'state' direct parts. It means only that this change must not affect the existence of the direct part itself.

There is no change in granularity or cardinality of direct parts within a 'state'.

Also, the 'state' must cover all the time interval between two successive cardinality changes.

The use of spatial direct parthood in 'state' definition means that a 'state' cannot overlap in space another 'state'.")
AnnotationAssertion(rdfs:comment <http://emmc.info/emmo-direct#EMMO_36c79456_e29c_400d_8bd3_0eedddb82652> "The usefulness of 'state' is that it makes it possible to describe the evolution in time of an 'existent' in terms of series of 'state'-s that can take into account the disappearance or appearance of parts within a 'physical'. 

A 'state' is a recognizable granularity level of matter, in the sense that its direct parts do not appear or disappear within its lifetime as it can be for a generic 'existent'.")
AnnotationAssertion(rdfs:comment <http://emmc.info/emmo-direct#EMMO_36c79456_e29c_400d_8bd3_0eedddb82652> "There is no change in granularity or cardinality of parts within a state.

The use of spatial direct parthood in state definition means that a state cannot overlap in space another state that is direct part of the same whole.")
AnnotationAssertion(rdfs:label <http://emmc.info/emmo-direct#EMMO_36c79456_e29c_400d_8bd3_0eedddb82652> "state"@en)
SubClassOf(<http://emmc.info/emmo-direct#EMMO_36c79456_e29c_400d_8bd3_0eedddb82652> <http://emmc.info/emmo-direct#EMMO_52211e5e_d767_4812_845e_eb6b402c476a>)
SubClassOf(<http://emmc.info/emmo-direct#EMMO_36c79456_e29c_400d_8bd3_0eedddb82652> ObjectUnionOf(<http://emmc.info/emmo-core#EMMO_0f795e3e_c602_4577_9a43_d5a231aa1360> ObjectSomeValuesFrom(<http://emmc.info/emmo-direct#EMMO_b2282816_b7a3_44c6_b2cb_3feff1ceb7fe> <http://emmc.info/emmo-direct#EMMO_52211e5e_d767_4812_845e_eb6b402c476a>)))

# Class: <http://emmc.info/emmo-direct#EMMO_52211e5e_d767_4812_845e_eb6b402c476a> (existent)

AnnotationAssertion(<http://emmc.info/emmo-core#EMMO_70fe84ff_99b6_4206_a9fc_9a8931836d84> <http://emmc.info/emmo-direct#EMMO_52211e5e_d767_4812_845e_eb6b402c476a> "A 'item' which is a 'state' or made only of 'state' temporal direct parts.")
AnnotationAssertion(rdfs:comment <http://emmc.info/emmo-direct#EMMO_52211e5e_d767_4812_845e_eb6b402c476a> "'existent' is the most important class to be used for representing real world objects under a reductionistic perspective (i.e. objects come from the composition of sub-part objects). 

'existent' class collects all individuals that stand for real world objects that can be structured in temporal sub-parts of constant mereological cardinality (i.e. number of parts) through the temporal direct parthood, that provides a way to axiomatize tassellation principles for a specific whole class, and non-transitivity to retain the granularity levels.

e.g. a car, a supersaturated gas with nucleating nanoparticles, an atom that becomes ionized and then recombines with an electron.")
AnnotationAssertion(rdfs:comment <http://emmc.info/emmo-direct#EMMO_52211e5e_d767_4812_845e_eb6b402c476a> "IMPORTANT:
if we agree that every item can be partitioned in time into 'state'-s with constant cardinality, then 'existent' is conincident with 'item'.")
AnnotationAssertion(rdfs:comment <http://emmc.info/emmo-direct#EMMO_52211e5e_d767_4812_845e_eb6b402c476a> "ex-sistere (latin): to stay (to persist through time) outside others of the same type (to be distinct from the rest).")
AnnotationAssertion(rdfs:label <http://emmc.info/emmo-direct#EMMO_52211e5e_d767_4812_845e_eb6b402c476a> "existent"@en)
SubClassOf(<http://emmc.info/emmo-direct#EMMO_52211e5e_d767_4812_845e_eb6b402c476a> <http://emmc.info/emmo-core#EMMO_c5ddfdba_c074_4aa4_ad6b_1ac4942d300d>)
SubClassOf(<http://emmc.info/emmo-direct#EMMO_52211e5e_d767_4812_845e_eb6b402c476a> ObjectUnionOf(<http://emmc.info/emmo-direct#EMMO_36c79456_e29c_400d_8bd3_0eedddb82652> ObjectSomeValuesFrom(<http://emmc.info/emmo-direct#EMMO_65a2c5b8_e4d8_4a51_b2f8_e55effc0547d> <http://emmc.info/emmo-direct#EMMO_36c79456_e29c_400d_8bd3_0eedddb82652>)))
SubClassOf(<http://emmc.info/emmo-direct#EMMO_52211e5e_d767_4812_845e_eb6b402c476a> ObjectAllValuesFrom(<http://emmc.info/emmo-direct#EMMO_65a2c5b8_e4d8_4a51_b2f8_e55effc0547d> <http://emmc.info/emmo-direct#EMMO_36c79456_e29c_400d_8bd3_0eedddb82652>))


)