<?xml version="1.0"?>
<rdf:RDF xmlns="http://emmo.info/emmo/top/perspectives#"
     xml:base="http://emmo.info/emmo/top/perspectives"
     xmlns:owl="http://www.w3.org/2002/07/owl#"
     xmlns:rdf="http://www.w3.org/1999/02/22-rdf-syntax-ns#"
     xmlns:xml="http://www.w3.org/XML/1998/namespace"
     xmlns:xsd="http://www.w3.org/2001/XMLSchema#"
     xmlns:rdfs="http://www.w3.org/2000/01/rdf-schema#"
     xmlns:annotations="http://emmo.info/emmo/top/annotations#">
    <owl:Ontology rdf:about="http://emmo.info/emmo/top/perspectives">
        <owl:versionIRI rdf:resource="http://emmo.info/emmo/1.0.0/top/perspectives"/>
        <owl:imports rdf:resource="http://emmo.info/emmo/1.0.0/top/physical"/>
        <annotations:EMMO_5525a055_dda5_4556_8b91_f0d22fa676cc>EMMO is released under a Creative Commons license Attribution 4.0 International (CC BY 4.0)

https://creativecommons.org/licenses/by/4.0/legalcode</annotations:EMMO_5525a055_dda5_4556_8b91_f0d22fa676cc>
        <annotations:EMMO_cd5fb112_7ee7_4120_a35d_3ca3e6c3f4ab>Emanuele Ghedini (University of Bologna, IT)
Gerhard Goldbeck (GCL Ltd, UK)
Adham Hashibon (Fraunhofer IWM, DE)
Georg Schmitz (Access, DE)
Jesper Friis (SINTEF, NO)</annotations:EMMO_cd5fb112_7ee7_4120_a35d_3ca3e6c3f4ab>
        <rdfs:comment xml:lang="en">Contacts:
Gerhard Goldbeck
Goldbeck Consulting Ltd (UK)
email: gerhard@goldbeck-consulting.com

Emanuele Ghedini
University of Bologna (IT)
email: emanuele.ghedini@unibo.it</rdfs:comment>
        <rdfs:comment>European Materials and Modelling Ontology (EMMO)

EMMO is a multidisciplinary effort to develop a standard representational framework (the ontology) based on current materials modelling knowledge, including physical sciences, analytical philosophy and information and communication technologies. 

It provides the connection between the physical world, materials characterisation world and materials modelling world.</rdfs:comment>
        <rdfs:comment>The EMMO requires FacT++ reasoner plugin in order to visualize all inferences and class hierarchy (ctrl+R hotkey in Protege).</rdfs:comment>
        <owl:versionInfo>The European Materials Modelling Ontology

Version 1.0.0</owl:versionInfo>
    </owl:Ontology>
    


    <!-- 
    ///////////////////////////////////////////////////////////////////////////////////////
    //
    // Object Properties
    //
    ///////////////////////////////////////////////////////////////////////////////////////
     -->

    


    <!-- http://emmo.info/emmo/top/perspectives#EMMO_ae2d1a96_bfa1_409a_a7d2_03d69e8a125a -->

    <owl:ObjectProperty rdf:about="http://emmo.info/emmo/top/perspectives#EMMO_ae2d1a96_bfa1_409a_a7d2_03d69e8a125a">
        <rdfs:subPropertyOf rdf:resource="http://emmo.info/emmo/top/mereotopology#EMMO_17e27c22_37e1_468c_9dd7_95e137f73e7f"/>
        <rdfs:domain rdf:resource="http://emmo.info/emmo/top/perspectives#EMMO_43e9a05d_98af_41b4_92f6_00f79a09bfce"/>
        <rdfs:range rdf:resource="http://emmo.info/emmo/top/perspectives#EMMO_49804605_c0fe_4538_abda_f70ba1dc8a5d"/>
        <annotations:EMMO_967080e5_2f42_4eb2_a3a9_c58143e835f9>The relation between a process and an object participating to it.</annotations:EMMO_967080e5_2f42_4eb2_a3a9_c58143e835f9>
        <rdfs:comment>Participation is a parthood relation: you must be part (and then be connected) of the process to contribute to it.</rdfs:comment>
        <rdfs:comment>Participation is not under direct parthood since a process is not strictly related to reductionism, but it&apos;s a way to categorize temporal regions by the interpreters.</rdfs:comment>
        <rdfs:label xml:lang="en">hasParticipant</rdfs:label>
    </owl:ObjectProperty>
    


    <!-- http://emmo.info/emmo/top/perspectives#EMMO_c5aae418_1622_4d02_93c5_21159e28e6c1 -->

    <owl:ObjectProperty rdf:about="http://emmo.info/emmo/top/perspectives#EMMO_c5aae418_1622_4d02_93c5_21159e28e6c1">
        <rdfs:subPropertyOf rdf:resource="http://emmo.info/emmo/top/mereotopology#EMMO_9380ab64_0363_4804_b13f_3a8a94119a76"/>
        <rdfs:subPropertyOf rdf:resource="http://emmo.info/emmo/top/perspectives#EMMO_ae2d1a96_bfa1_409a_a7d2_03d69e8a125a"/>
        <rdfs:label xml:lang="en">hasProperParticipant</rdfs:label>
    </owl:ObjectProperty>
    


    <!-- 
    ///////////////////////////////////////////////////////////////////////////////////////
    //
    // Classes
    //
    ///////////////////////////////////////////////////////////////////////////////////////
     -->

    


    <!-- http://emmo.info/emmo/top/perspectives#EMMO_0277f24a_ea7f_4917_81b7_fb0406c8fc62 -->

    <owl:Class rdf:about="http://emmo.info/emmo/top/perspectives#EMMO_0277f24a_ea7f_4917_81b7_fb0406c8fc62">
        <owl:equivalentClass>
            <owl:Class>
                <owl:unionOf rdf:parseType="Collection">
                    <rdf:Description rdf:about="http://emmo.info/emmo/top/perspectives#EMMO_43e9a05d_98af_41b4_92f6_00f79a09bfce"/>
                    <rdf:Description rdf:about="http://emmo.info/emmo/top/perspectives#EMMO_49804605_c0fe_4538_abda_f70ba1dc8a5d"/>
                </owl:unionOf>
            </owl:Class>
        </owl:equivalentClass>
        <rdfs:subClassOf rdf:resource="http://emmo.info/emmo/top/perspectives#EMMO_49267eba_5548_4163_8f36_518d65b583f9"/>
        <annotations:EMMO_967080e5_2f42_4eb2_a3a9_c58143e835f9>A union of classes that categorize physicals under a holistic perspective, meaning that the interest is on the whole 4D object (process) and the role of its spatial parts (participants) without going further into its subparts.</annotations:EMMO_967080e5_2f42_4eb2_a3a9_c58143e835f9>
        <rdfs:comment>Holism (from Greek ὅλος holos &quot;all, whole, entire&quot;)</rdfs:comment>
        <rdfs:label xml:lang="en">Holistic</rdfs:label>
    </owl:Class>
    


    <!-- http://emmo.info/emmo/top/perspectives#EMMO_15db234d_ecaf_4715_9838_4b4ec424fb13 -->

    <owl:Class rdf:about="http://emmo.info/emmo/top/perspectives#EMMO_15db234d_ecaf_4715_9838_4b4ec424fb13">
        <owl:equivalentClass>
            <owl:Class>
                <owl:unionOf rdf:parseType="Collection">
                    <rdf:Description rdf:about="http://emmo.info/emmo/top/perspectives#EMMO_36c79456_e29c_400d_8bd3_0eedddb82652"/>
                    <rdf:Description rdf:about="http://emmo.info/emmo/top/perspectives#EMMO_52211e5e_d767_4812_845e_eb6b402c476a"/>
                </owl:unionOf>
            </owl:Class>
        </owl:equivalentClass>
        <rdfs:subClassOf rdf:resource="http://emmo.info/emmo/top/perspectives#EMMO_49267eba_5548_4163_8f36_518d65b583f9"/>
        <annotations:EMMO_967080e5_2f42_4eb2_a3a9_c58143e835f9>A class devoted to categorize &apos;Physical&apos;-s according to their granularity relations, first in terms of time evolution (Existent) and then in terms of their composition (State), up to the spatial a-tomistic element (Elementary).</annotations:EMMO_967080e5_2f42_4eb2_a3a9_c58143e835f9>
        <rdfs:label xml:lang="en">Reductionistic</rdfs:label>
    </owl:Class>
    


    <!-- http://emmo.info/emmo/top/perspectives#EMMO_36c79456_e29c_400d_8bd3_0eedddb82652 -->

    <owl:Class rdf:about="http://emmo.info/emmo/top/perspectives#EMMO_36c79456_e29c_400d_8bd3_0eedddb82652">
        <annotations:EMMO_967080e5_2f42_4eb2_a3a9_c58143e835f9>A &apos;Physical&apos; which is a tessellation of other &apos;Physical&apos; spatial direct parts.</annotations:EMMO_967080e5_2f42_4eb2_a3a9_c58143e835f9>
        <annotations:EMMO_b432d2d5_25f4_4165_99c5_5935a7763c1a>e.g. the existent in my glass is declared at t = t_start as made of two direct parts: the ice and the water. It will continue to exists as state as long as the ice is completely melt at t = t_end. The new state will be completely made of water. Between t_start and t_end there is an exchange of molecules between the ice and the water, but this does not affect the existence of the two states.

If we partition the existent in my glass as ice surrounded by several molecules (we do not use the object water as direct part) then the appearance of a molecule coming from the ice will cause a state to end and another state to begin.</annotations:EMMO_b432d2d5_25f4_4165_99c5_5935a7763c1a>
        <rdfs:comment>Direct partitions declaration is a choice of the ontologist that choses the classes to be used as direct parts, according to its own world view.

A &apos;State&apos; can always be direct partitioned in &apos;Elementary&apos;-s and &apos;Void&apos; or &apos;Physical&apos;.

e.g. the water in my glass can be seen as a single object without declaring direct parts, or as made of H2O molecules direct parts.</rdfs:comment>
        <rdfs:comment>The definition of &apos;State&apos; implies that its spatial direct parts (i.e. &apos;physicals&apos;) are not gained or lost during its temporal extension (they exist from the left to the right side of the time interval), so that the granularity of a &apos;state&apos; is constant.

This does not mean that there cannot be a change in the internal structure of the &apos;State&apos; direct parts. It means only that this change must not affect the existence of the direct part itself.

There is no change in granularity or cardinality of direct parts of a &apos;State&apos;.

The use of spatial direct parthood in &apos;State&apos; definition means that a &apos;State&apos; cannot overlap in space another &apos;State&apos;.</rdfs:comment>
        <rdfs:comment>The usefulness of &apos;state&apos; is that it makes it possible to describe the evolution in time of an &apos;existent&apos; in terms of series of &apos;state&apos;-s that can take into account the disappearance or appearance of parts within a &apos;physical&apos;. 

A &apos;state&apos; is a recognizable granularity level of matter, in the sense that its direct parts do not appear or disappear within its lifetime as it can be for a generic &apos;existent&apos;.</rdfs:comment>
        <rdfs:comment>There is no change in granularity or cardinality of parts within a state.

The use of spatial direct parthood in state definition means that a state cannot overlap in space another state that is direct part of the same whole.</rdfs:comment>
        <rdfs:label xml:lang="en">State</rdfs:label>
    </owl:Class>
    


    <!-- http://emmo.info/emmo/top/perspectives#EMMO_43e9a05d_98af_41b4_92f6_00f79a09bfce -->

    <owl:Class rdf:about="http://emmo.info/emmo/top/perspectives#EMMO_43e9a05d_98af_41b4_92f6_00f79a09bfce">
        <rdfs:subClassOf rdf:resource="http://emmo.info/emmo/top/physical#EMMO_c5ddfdba_c074_4aa4_ad6b_1ac4942d300d"/>
        <rdfs:subClassOf>
            <owl:Restriction>
                <owl:onProperty rdf:resource="http://emmo.info/emmo/top/perspectives#EMMO_ae2d1a96_bfa1_409a_a7d2_03d69e8a125a"/>
                <owl:someValuesFrom rdf:resource="http://emmo.info/emmo/top/perspectives#EMMO_49804605_c0fe_4538_abda_f70ba1dc8a5d"/>
            </owl:Restriction>
        </rdfs:subClassOf>
        <annotations:EMMO_967080e5_2f42_4eb2_a3a9_c58143e835f9>A temporal part of a &apos;physical&apos; that identifies a particular type of evolution in time.</annotations:EMMO_967080e5_2f42_4eb2_a3a9_c58143e835f9>
        <rdfs:comment>A &apos;Process&apos; is always a &apos;Physical&apos;, since a &apos;Void&apos; does not have elements that evolves in time.</rdfs:comment>
        <rdfs:comment>A &apos;Process&apos; is defined as a temporal part of a &apos;Physical&apos; that is categorized according to an EMMO user that recognizes a particular type of evolution in time of the real world object.

Following the common definition of process, every &apos;Physical&apos; should be a process, since every 4D object always has a time dimension. 

However, in the EMMO we restrict the meaning of the word process to &apos;Physical&apos;-s whose evolution in time have a particular meaning for the ontologist.

A &apos;Process&apos; is not only something that unfolds in time (which is automatically represented in a 4D ontology), but something that has a meaning for the ontologist, i.e. that the ontologist can separate from the rest of the 4D physical for any reason.</rdfs:comment>
        <rdfs:label xml:lang="en">Process</rdfs:label>
    </owl:Class>
    


    <!-- http://emmo.info/emmo/top/perspectives#EMMO_49267eba_5548_4163_8f36_518d65b583f9 -->

    <owl:Class rdf:about="http://emmo.info/emmo/top/perspectives#EMMO_49267eba_5548_4163_8f36_518d65b583f9">
        <rdfs:subClassOf rdf:resource="http://emmo.info/emmo/top/physical#EMMO_c5ddfdba_c074_4aa4_ad6b_1ac4942d300d"/>
        <annotations:EMMO_967080e5_2f42_4eb2_a3a9_c58143e835f9>The class of individuals that stand for real world objects according to a specific representational perspective.</annotations:EMMO_967080e5_2f42_4eb2_a3a9_c58143e835f9>
        <rdfs:label xml:lang="en">Perspective</rdfs:label>
    </owl:Class>
    


    <!-- http://emmo.info/emmo/top/perspectives#EMMO_49804605_c0fe_4538_abda_f70ba1dc8a5d -->

    <owl:Class rdf:about="http://emmo.info/emmo/top/perspectives#EMMO_49804605_c0fe_4538_abda_f70ba1dc8a5d">
        <rdfs:subClassOf>
            <owl:Restriction>
                <owl:onProperty>
                    <rdf:Description>
                        <owl:inverseOf rdf:resource="http://emmo.info/emmo/top/perspectives#EMMO_ae2d1a96_bfa1_409a_a7d2_03d69e8a125a"/>
                    </rdf:Description>
                </owl:onProperty>
                <owl:someValuesFrom rdf:resource="http://emmo.info/emmo/top/perspectives#EMMO_43e9a05d_98af_41b4_92f6_00f79a09bfce"/>
            </owl:Restriction>
        </rdfs:subClassOf>
        <annotations:EMMO_967080e5_2f42_4eb2_a3a9_c58143e835f9>A portion of a &apos;Process&apos; that participates to the process with a specific role.</annotations:EMMO_967080e5_2f42_4eb2_a3a9_c58143e835f9>
        <rdfs:comment>In the EMMO the relation of participation to a process falls under mereotopology.</rdfs:comment>
        <rdfs:label xml:lang="en">Participant</rdfs:label>
    </owl:Class>
    


    <!-- http://emmo.info/emmo/top/perspectives#EMMO_52211e5e_d767_4812_845e_eb6b402c476a -->

    <owl:Class rdf:about="http://emmo.info/emmo/top/perspectives#EMMO_52211e5e_d767_4812_845e_eb6b402c476a">
        <annotations:EMMO_967080e5_2f42_4eb2_a3a9_c58143e835f9>A &apos;Physical&apos; which is a tessellation of &apos;State&apos; temporal direct parts.</annotations:EMMO_967080e5_2f42_4eb2_a3a9_c58143e835f9>
        <rdfs:comment>&apos;Existent&apos; is the EMMO class to be used for representing real world physical objects under a reductionistic (i.e. objects come from the composition of sub-part objects, both in time and space) and epistemological pluralistic (i.e. objects definitions are interpreter dependent) perspectives . 

&apos;Existent&apos; class collects all individuals that stand for physical objects that can be structured in well defined temporal sub-parts called states, through the temporal direct parthood relation.

This class provides a first granularity hierarchy in time, and a way to axiomatize tessellation principles for a specific whole with a non-transitivity relation (direct parthood) that helps to retain the granularity levels.

e.g. a car, a supersaturated gas with nucleating nanoparticles, an atom that becomes ionized and then recombines with an electron.</rdfs:comment>
        <rdfs:comment>An &apos;Existent&apos; individual stands for a real world object for which the ontologist can provide univocal tessellation in time.

By definition, the tiles are represented by &apos;State&apos;-s individual.

Tiles are related to the &apos;Existent&apos; through temporal direct parthood, enforcing non-transitivity and inverse-functionality.</rdfs:comment>
        <rdfs:comment>Being hasTemporalDirectPart a proper parthood relation, there cannot be &apos;Existent&apos; made of a single &apos;State&apos;.</rdfs:comment>
        <rdfs:comment>ex-sistere (latin): to stay (to persist through time) outside others of the same type (to be distinct from the rest).</rdfs:comment>
        <rdfs:label xml:lang="en">Existent</rdfs:label>
    </owl:Class>
    


    <!-- http://emmo.info/emmo/top/perspectives#EMMO_649bf97b_4397_4005_90d9_219755d92e34 -->

    <owl:Class rdf:about="http://emmo.info/emmo/top/perspectives#EMMO_649bf97b_4397_4005_90d9_219755d92e34">
        <rdfs:subClassOf rdf:resource="http://emmo.info/emmo/top/perspectives#EMMO_49267eba_5548_4163_8f36_518d65b583f9"/>
        <annotations:EMMO_967080e5_2f42_4eb2_a3a9_c58143e835f9>A &apos;Physical&apos; which stands for a real world object that can stimulate a perception (e.g. a mental impression, the excitation of a sensor) to an interpreter (human or non-human).</annotations:EMMO_967080e5_2f42_4eb2_a3a9_c58143e835f9>
        <annotations:EMMO_b432d2d5_25f4_4165_99c5_5935a7763c1a>A line scratched on a surface.
A sound.
A smell.
The word &apos;cat&apos; and the sound of the word &apos;cat&apos; (the first one is graphical and the second acoustical).</annotations:EMMO_b432d2d5_25f4_4165_99c5_5935a7763c1a>
        <annotations:EMMO_b432d2d5_25f4_4165_99c5_5935a7763c1a>The meta-semiotic process:
I see a cloud in the sky. Since I&apos;m an EMMO ontologist, I create an individual named Cloud under the &apos;Impression&apos; class.  This semiotic process occurs at meta-level: it&apos;s how I use the EMMO as tool for a direct representation of the world.

The semiotic process within EMMO:
My friend looks at the same cloud and says: &quot;It is an elephant&quot;.
I use the EMMO to record this experience by declaring:
    - my friend as MyFriend individual, belonging to &apos;Interpreter&apos; classes
    - the sound of the word &quot;elephant&quot; as an acoustical impression individual named ElephantWord, belonging to &apos;Impression&apos;
    - a relation hasSign between Cloud and ElephantWord, that makes ElephantWord also belonging to &apos;Sign&apos; class and Cloud belonging also to &apos;Object&apos; class
    - a &apos;Semiosis&apos; individual called MyFriendElephantCloud that hasParticipant: Cloud, ElephantWord and MyFriend, respectively as object, sign and interpreter.</annotations:EMMO_b432d2d5_25f4_4165_99c5_5935a7763c1a>
        <rdfs:comment>&apos;Impression&apos; includes real world objects that:
- are part of a communication system (e.g. words, speech, alphabets)
- are not part of a communication system, but can be identified and referred by an interpreter</rdfs:comment>
        <rdfs:comment>An &apos;Impression&apos; is a meta-object, meaning that is addressed by the ontologist (the meta-interpreter) in a meta-semiotic process occurring outside the EMMO.

An &apos;Impression&apos; becomes an &apos;Object&apos;, when it is part of a &apos;Semiotic&apos; process described by the ontologist through the EMMO.</rdfs:comment>
        <rdfs:comment>From Latin impressionem: &quot;a pressing into, onset, attack,&quot; figuratively &quot;a perception, mental impression&quot;.

Literally &quot;a pressing into&quot; from Latin imprimere &quot;press into or upon&quot;.</rdfs:comment>
        <rdfs:comment>This class is the most general superclass for the categorization of real world objects that are recognizable by an interpreter (agent).

An &apos;Impression&apos; can stand for something else in a semiotic process (acting as sign or as object). 

However, an impression is not necessarily a &apos;sign&apos; (e.g. a line sketched on a blackboard is a recognizable &apos;impression&apos; but it may stand for nothing).</rdfs:comment>
        <rdfs:label xml:lang="en">Phenomenic</rdfs:label>
    </owl:Class>
    


    <!-- http://emmo.info/emmo/top/perspectives#EMMO_98ada9d8_f1c8_4f13_99b5_d890f5354152 -->

    <owl:Class rdf:about="http://emmo.info/emmo/top/perspectives#EMMO_98ada9d8_f1c8_4f13_99b5_d890f5354152">
        <rdfs:subClassOf rdf:resource="http://emmo.info/emmo/top/perspectives#EMMO_49267eba_5548_4163_8f36_518d65b583f9"/>
        <rdfs:label xml:lang="en">Physics</rdfs:label>
    </owl:Class>
</rdf:RDF>



<!-- Generated by the OWL API (version 4.5.9.2019-02-01T07:24:44Z) https://github.com/owlcs/owlapi -->

